\begin{enumerate}[label=\thechapter.\arabic*,ref=\thechapter.\theenumi]
\numberwithin{equation}{enumi}
\numberwithin{figure}{enumi}
\numberwithin{table}{enumi}
\item Laplace Transform of Partial Differentials\\
Let a function $y\brak{x,t}$ be defined for all $t>0$ and assumed to be bounded. Appling Laplace transform in t considering x as a parameter,
\begin{align}
 \mathcal{L}\brak{y\brak{x,t}} &= \int_{0}^{\infty}e^{-st}y\brak{x,t}dt\\
 &= Y\brak{x,s}
\end{align}
Let $\dfrac{\partial y\brak{x,t}}{\partial t}$ be $y_t\brak{x,t}$ and $\dfrac{\partial y\brak{x,t}}{\partial x}$ be $y_x\brak{x,t}$, then
\begin{align}
 \mathcal{L}\brak{y_t\brak{x,t}} &= \int_{0}^{\infty}e^{-st}y_t\brak{x,t}dt\\
 &= \left. e^{-st}y\brak{x,t}\right|_{0}^{\infty} + s\int_{0}^{\infty}e^{-st} y\brak{x,t} dt\\
 &= sY\brak{x,s} - y\brak{x,0} \label{L(y_t(x,t))}\\
 \mathcal{L}\brak{y_x\brak{x,t}} &= \int_{0}^{\infty}e^{-st}y_x\brak{x,t}dt\\
 &= \dfrac{d}{dx}\int_{0}^{\infty}e^{-st}y\brak{x,t}dt \label{L(y_x(x,t))}\\
 &= \dfrac{dY\brak{x,s}}{dx}
\end{align}

\item Laplace transform of integrals:\\
Let the function defined as $y(t) = \int_0^t f(u) du$ for all $t > 0$\\
Laplace transform of y(t) in t 
\begin{align}
    \mathcal{L} \brak{y(t)} &= \int_0^{\infty} e^{-st} y(t) dt\\
    &= \int_0^{\infty} e^{-st} \int_0^t f(u) du dt\\
    &= \int_0^t f(u) du \sbrak{- \frac{e^{-st}}{s}}_0^{\infty} + \int_0^{\infty} \frac{e^{-st}}{s} f(t) dt\\
    &= \frac{F(s)}{s}
\end{align}

\end{enumerate}
